% !TEX=../main.tex
\documentclass[../main.tex]{subfiles}

% ==============================================================
% initial point 1.2 1.2 case
% =============================================================
\newcommand{\insertfigures}[5]{
\begin{figure}[ht]
\begin{multicols}{2}
  \begin{subfigure}{.45\textwidth}
    \includegraphics[width=\linewidth]{#1} \par
  \caption{SteepestDescent}  
  \end{subfigure}
  \begin{subfigure}{.45\textwidth}
    \includegraphics[width=\linewidth]{#2} \par
    \caption{Newtons}
  \end{subfigure}
  \end{multicols} 
  \begin{multicols}{2}
  \begin{subfigure}{.45\textwidth}
    \includegraphics[width=\linewidth]{#3} \par
    \caption{SR1}
  \end{subfigure}
  \begin{subfigure}{.45\textwidth}
    \includegraphics[width=\linewidth]{#4} \par
    \caption{BFGS}
  \end{subfigure}
\end{multicols}
  \caption{#5}
\end{figure}
}

\begin{document}

% ======================================== 
% initial point [1.2, 1.2]
% ========================================
\insertfigures
{figures/a_SteepestDescent_[1.2, 1.2].png}
{figures/a_Newtons_[1.2, 1.2].png}
{figures/a_SR1_[1.2, 1.2].png}
{figures/a_BFGS_[1.2, 1.2].png}
{$f(x, y)=(x+2y-6)^2 + (2x+y-6)^2$}

\insertfigures
{figures/b_SteepestDescent_[1.2, 1.2].png}
{figures/b_Newtons_[1.2, 1.2].png}
{figures/b_SR1_[1.2, 1.2].png}
{figures/b_BFGS_[1.2, 1.2].png}
{$(x, y)=50*(y-x^2)^2 + (1-x)^2$}

\insertfigures
{figures/c_SteepestDescent_[1.2, 1.2].png}
{figures/c_Newtons_[1.2, 1.2].png}
{figures/c_SR1_[1.2, 1.2].png}
{figures/c_BFGS_[1.2, 1.2].png}
{$f(x, y)=(1.5-x+xy)^2 + (2.25-x+xy^2)^2 + (2.625 - x+ xy^3)^2$}

% ======================================== 
% initial point [5.6, -1.2]
% ========================================
\insertfigures
{figures/a_SteepestDescent_[5.6,-1.2].png}
{figures/a_Newtons_[5.6,-1.2].png}
{figures/a_SR1_[5.6,-1.2].png}
{figures/a_BFGS_[5.6,-1.2].png}
{$f(x, y)=(x+2y-6)^2 + (2x+y-6)^2$}

\insertfigures
{figures/b_SteepestDescent_[5.6,-1.2].png}
{figures/b_Newtons_[5.6,-1.2].png}
{figures/b_SR1_[5.6,-1.2].png}
{figures/b_BFGS_[5.6,-1.2].png}
{$(x, y)=50*(y-x^2)^2 + (1-x)^2$}

\insertfigures
{figures/c_SteepestDescent_[5.6,-1.2].png}
{figures/c_Newtons_[5.6,-1.2].png}
{figures/c_SR1_[5.6,-1.2].png}
{figures/c_BFGS_[5.6,-1.2].png}
{$f(x, y)=(1.5-x+xy)^2 + (2.25-x+xy^2)^2 + (2.625 - x+ xy^3)^2$}

% ======================================== 
% initial point [-3.5, 2.3]
% ========================================
\insertfigures
{figures/a_SteepestDescent_[-3.5,2.3].png}
{figures/a_Newtons_[-3.5,2.3].png}
{figures/a_SR1_[-3.5,2.3].png}
{figures/a_BFGS_[-3.5,2.3].png}
{$f(x, y)=(x+2y-6)^2 + (2x+y-6)^2$}

\insertfigures
{figures/b_SteepestDescent_[-3.5,2.3].png}
{figures/b_Newtons_[-3.5,2.3].png}
{figures/b_SR1_[-3.5,2.3].png}
{figures/b_BFGS_[-3.5,2.3].png}
{$(x, y)=50*(y-x^2)^2 + (1-x)^2$}

% ======================================== 
% initial point [10.5,-8.3]
% ========================================
\insertfigures
{figures/a_SteepestDescent_[10.5,-8.3].png}
{figures/a_Newtons_[10.5,-8.3].png}
{figures/a_SR1_[10.5,-8.3].png}
{figures/a_BFGS_[10.5,-8.3].png}
{$f(x, y)=(x+2y-6)^2 + (2x+y-6)^2$}

\end{document}